MyBase.v
@@ -45,7 +45,7 @@ Ltac elim_sumbools dec := repeat match goal with
                                  | H : context[dec _ _] |- _ => move/sumboolP in H
                                  end.
 
-Ltac split_iff := match goal with H: iff _ _ |- _ => case H end.
+Ltac split_iff := match goal with H: iff _ _ |- _ => case H; clear H end.
 Ltac split_iffs := repeat split_iff.
 
 Ltac program_equiv_case_analysis :=
@@ -58,7 +58,7 @@ Ltac program_equiv_case_analysis :=
 Ltac program_equiv := repeat program_equiv_case_analysis.
 
 Ltac done_rec := 
-  intros; subst; simpl in *; InvertReflections; split_iffs; (
+  intros; subst; simpl in *; (
     match goal with
     | H : _ |- ~ _ => (progress inversion 1); done_rec
     | R : reflect ?e _, H : ?e |- _ => move/R in H; done_rec
@@ -68,7 +68,7 @@ Ltac done_rec :=
     || ((progress ApplyOneHypothesis); done_rec)
     || (econstructor; done_rec)).
 
-Ltac done := subst; simpl in *; repeat (program_equiv; intro); done_rec.
+Ltac done := subst; simpl in *; InvertReflections; split_iffs; repeat (program_equiv; intro); done_rec.
 
 Ltac inv H := inversion H; subst; clear H.
 
